factor out Bind_ lemmas

src/FlatToRiscv.v
@@ -19,6 +19,7 @@ Require Import Coq.Logic.FunctionalExtensionality.
 Require Import riscv.InstructionCoercions.
 Require Import riscv.Utility.
 Require Import compiler.StateCalculus.
+Require Import compiler.AxiomaticRiscv.
 
 Local Open Scope ilist_scope.
 
@@ -83,24 +84,12 @@ Section FlatToRiscv.
   Context {state: Type}.
   Context {stateMap: Map state Register (word wXLEN)}.
 
-  Instance State_is_RegisterFile: RegisterFile state Register (word wXLEN) := {|
-    getReg rf r := match get rf r with
-                   | Some v => v
-                   | None => $0
-                   end;
-    setReg := put;
-    initialRegs := empty;
-  |}.
-
   (* assumes generic translate and raiseException functions *)
   Context {RVS: @RiscvState (OState RiscvMachine) (word wXLEN) _ _ IsRiscvMachine}.  
 
-  Definition RiscvMachine := @RiscvMachine Bw (mem wXLEN) state.
+  Local Notation RiscvMachine := (@RiscvMachine Bw (mem wXLEN) state).
 
   Ltac state_calc := state_calc_generic (@name TestFlatImp.ZName) (word wXLEN).
-
-  (* Note: Register 0 is not considered valid because it cannot be written *)
-  Definition valid_register(r: Register): Prop := (0 < r < 32)%Z.
 
   (* This phase assumes that register allocation has already been done on the FlatImp
      level, and expects the following to hold: *)
@@ -841,45 +830,6 @@ Section FlatToRiscv.
     change $0 with (wzero wXLEN).
     ring.
   Qed. 
-  
-  Lemma Bind_getRegister0: forall {A: Type} (f: word wXLEN -> OState RiscvMachine A),
-      Bind (getRegister Register0) f = f $0.
-  Proof.
-    intros. reflexivity.
-  Qed.
-
-  Lemma Bind_getRegister: forall {A: Type} x
-                                 (f: word wXLEN -> OState RiscvMachine A)
-                                 (initialL: RiscvMachine),
-      valid_register x ->
-      execState (Bind (getRegister x) f) initialL =
-      execState (f (getReg initialL.(core).(registers) x)) initialL.
-  Proof.
-    intros. simpl.
-    destruct_one_match.
-    - exfalso. unfold valid_register, Register0 in *. omega.
-    - reflexivity.
-  Qed.
-
-  Lemma Bind_setRegister: forall {A: Type} x (v: word wXLEN)
-                                 (f: unit -> OState RiscvMachine A) (initialL: RiscvMachine),
-      valid_register x ->
-      execState (Bind (setRegister x v) f) initialL =
-      execState (f tt) (with_registers (setReg initialL.(core).(registers) x v) initialL).
-  Proof.
-    intros. simpl.
-    destruct_one_match.
-    - exfalso. unfold valid_register, Register0 in *. omega.
-    - reflexivity.
-  Qed.
-
-  Lemma Bind_setRegister0: forall {A: Type} (v: word wXLEN)
-                                 (f: unit -> OState RiscvMachine A) (initialL: RiscvMachine),
-      execState (Bind (setRegister Register0 v) f) initialL =
-      execState (f tt) initialL.
-  Proof.
-    intros. simpl. reflexivity.
-  Qed.
 
   (* Not sure if typechecking this ever finishes:
   Definition load_wXLEN: word wXLEN -> OState RiscvMachine (word wXLEN) :=
@@ -891,7 +841,6 @@ Section FlatToRiscv.
   Definition load_wXLEN: word wXLEN -> OState RiscvMachine (word wXLEN).
     set (lw := loadWord).
     set (ld := loadDouble).
-    unfold RiscvMachine in *.
     unfold State_is_RegisterFile in *.
     unfold RiscvBitWidths in *.
     unfold wXLEN in *.
@@ -910,7 +859,6 @@ Section FlatToRiscv.
     intros.
     unfold containsMem in *.
     specialize H0 with (1 := H).
-    unfold RiscvMachine in *.
     unfold State_is_RegisterFile in *.
     unfold containsMem, loadWordL, load_wXLEN in *.
     unfold bitwidth in *.
@@ -919,38 +867,6 @@ Section FlatToRiscv.
     inversions H;
     reflexivity.
   Qed.
-
-  Lemma Bind_getPC: forall {A: Type} (f: word wXLEN -> OState RiscvMachine A) (initialL: RiscvMachine),
-      execState (Bind getPC f) initialL =
-      execState (f initialL.(core).(pc)) initialL.
-  Proof.
-    intros. reflexivity.
-  Qed.
-
-  Lemma Bind_setPC: forall {A: Type} (v: word wXLEN)
-                                 (f: unit -> OState RiscvMachine A) (initialL: RiscvMachine),
-      execState (Bind (setPC v) f) initialL =
-      execState (f tt) (with_nextPC v initialL).
-  Proof.
-    intros. simpl. reflexivity.
-  Qed.
-  
-  Lemma Bind_step: forall {A: Type} (f: unit -> OState RiscvMachine A) m,
-      execState (Bind step f) m =
-      execState (f tt) (with_nextPC (m.(core).(nextPC) ^+ $4) (with_pc m.(core).(nextPC) m)).
-  Proof.
-    intros. reflexivity.
-  Qed.
-
-  Lemma execState_step: forall m,
-      execState step m = with_nextPC (m.(core).(nextPC) ^+ $4) (with_pc m.(core).(nextPC) m).
-  Proof.
-    intros. reflexivity.
-  Qed.
-  
-  Lemma execState_Return: forall {S A} (s: S) (a: A),
-      execState (Return a) s = s.
-  Proof. intros. reflexivity. Qed.
 
   Ltac do_get_set_Register :=
     repeat (
@@ -964,7 +880,7 @@ Section FlatToRiscv.
         rewrite? Bind_getPC;
         rewrite? Bind_setPC
       ).
-  
+
   Ltac prove_alu_def :=
     intros; clear; unfold wXLEN in *; unfold MachineWidthInst;
     destruct bitwidth; [unfold MachineWidth32 | unfold MachineWidth64]; reflexivity.
@@ -1244,12 +1160,18 @@ list2imem
       end.
 
   Ltac rewrite_reg_value :=
-    unfold getReg, State_is_RegisterFile;
-    let G1 := fresh "G1" in 
     match goal with
-    | G2: get ?st2 ?x = ?v, E: extends ?st1 ?st2 |- context [?gg] =>
-      match gg with
-      | get st1 x => assert (G1: gg = v) by (clear -G2 E; state_calc)
+    | |- context [getReg _ _] => idtac
+    | _ => fail 1 "wrong shape of goal"
+    end;
+    let G1 := fresh "G1" in
+    match goal with
+    | G2: get ?st2 ?x = ?v, E: extends ?st1 ?st2 |- context [@getReg ?RF ?R ?V ?TC ?st1 ?x] =>
+      let gg := constr:(@getReg RF R V TC st1 x) in
+      let gg' := eval unfold getReg, State_is_RegisterFile in gg in
+      change gg with gg';
+      match gg' with
+      | match ?gg'' with | _ => _ end => assert (G1: gg'' = v) by (clear -G2 E; state_calc)
       end
     end;
     rewrite G1.
@@ -1508,7 +1430,7 @@ list2imem
     pose proof @Bind_setRegister as Bind_setRegister.
     pose proof @Bind_load as Bind_load.
     unfold containsMem, Memory.read_mem, Memory.wXLEN_in_bytes, load_wXLEN in *.
-    unfold LwXLEN, bitwidth, State_is_RegisterFile, RiscvMachine, loadWordL in *.
+    unfold LwXLEN, bitwidth, loadWordL in *.
     destruct Bw eqn: EBw;
       (destruct_one_match_hyp; [|discriminate]);
       simpl in H2;
