src/AxiomaticRiscv.v
@@ -1,0 +1,125 @@
+Require Import lib.LibTacticsMin.
+Require Import riscv.util.Monads.
+Require Import compiler.Common.
+Require Import compiler.FlatImp.
+Require Import compiler.StateCalculus.
+Require Import bbv.DepEqNat.
+Require Import Coq.Lists.List.
+Import ListNotations.
+Require Import compiler.Op.
+Require Import compiler.ResMonad.
+Require Import riscv.Riscv.
+Require Import riscv.Minimal.
+Require Import riscv.FunctionMemory.
+Require Import compiler.runsToSatisfying.
+Require Import riscv.RiscvBitWidths.
+Require Import compiler.NameWithEq.
+Require Import Coq.Program.Tactics.
+Require Import Coq.Logic.FunctionalExtensionality.
+Require Import riscv.InstructionCoercions.
+Require Import riscv.Utility.
+Require Import compiler.StateCalculus.
+
+Local Open Scope ilist_scope.
+
+Set Implicit Arguments.
+
+
+Section AxiomaticRiscv.
+
+  Context {Bw: RiscvBitWidths}.
+
+  Context {state: Type}.
+  Context {stateMap: Map state Register (word wXLEN)}.
+
+  Instance State_is_RegisterFile: RegisterFile state Register (word wXLEN) := {|
+    getReg rf r := match get rf r with
+                   | Some v => v
+                   | None => $0
+                   end;
+    setReg := put;
+    initialRegs := empty;
+  |}.
+
+  (* assumes generic translate and raiseException functions *)
+  Context {RVS: @RiscvState (OState RiscvMachine) (word wXLEN) _ _ IsRiscvMachine}.  
+
+  (* Note: Register 0 is not considered valid because it cannot be written *)
+  Definition valid_register(r: Register): Prop := (0 < r < 32)%Z.
+
+  Local Notation RiscvMachine := (@RiscvMachine Bw (mem wXLEN) state).
+
+  Lemma Bind_getRegister0: forall {A: Type} (f: word wXLEN -> OState RiscvMachine A),
+      Bind (getRegister Register0) f = f $0.
+  Proof.
+    intros. reflexivity.
+  Qed.
+
+  Lemma Bind_getRegister: forall {A: Type} x
+                                 (f: word wXLEN -> OState RiscvMachine A)
+                                 (initialL: RiscvMachine),
+      valid_register x ->
+      execState (Bind (getRegister x) f) initialL =
+      execState (f (getReg initialL.(core).(registers) x)) initialL.
+  Proof.
+    intros. simpl.
+    destruct_one_match.
+    - exfalso. unfold valid_register, Register0 in *. omega.
+    - reflexivity.
+  Qed.
+
+  Lemma Bind_setRegister: forall {A: Type} x (v: word wXLEN)
+                                 (f: unit -> OState RiscvMachine A) (initialL: RiscvMachine),
+      valid_register x ->
+      execState (Bind (setRegister x v) f) initialL =
+      execState (f tt) (with_registers (setReg initialL.(core).(registers) x v) initialL).
+  Proof.
+    intros. simpl.
+    destruct_one_match.
+    - exfalso. unfold valid_register, Register0 in *. omega.
+    - reflexivity.
+  Qed.
+
+  Lemma Bind_setRegister0: forall {A: Type} (v: word wXLEN)
+                                 (f: unit -> OState RiscvMachine A) (initialL: RiscvMachine),
+      execState (Bind (setRegister Register0 v) f) initialL =
+      execState (f tt) initialL.
+  Proof.
+    intros. simpl. reflexivity.
+  Qed.
+
+  Lemma Bind_getPC: forall {A: Type} (f: word wXLEN -> OState RiscvMachine A) (initialL: RiscvMachine),
+      execState (Bind getPC f) initialL =
+      execState (f initialL.(core).(pc)) initialL.
+  Proof.
+    intros. reflexivity.
+  Qed.
+
+  Lemma Bind_setPC: forall {A: Type} (v: word wXLEN)
+                                 (f: unit -> OState RiscvMachine A) (initialL: RiscvMachine),
+      execState (Bind (setPC v) f) initialL =
+      execState (f tt) (with_nextPC v initialL).
+  Proof.
+    intros. simpl. reflexivity.
+  Qed.
+  
+  Lemma Bind_step: forall {A: Type} (f: unit -> OState RiscvMachine A) m,
+      execState (Bind step f) m =
+      execState (f tt) (with_nextPC (m.(core).(nextPC) ^+ $4) (with_pc m.(core).(nextPC) m)).
+  Proof.
+    intros. reflexivity.
+  Qed.
+
+  Lemma execState_step: forall m,
+      execState step m = with_nextPC (m.(core).(nextPC) ^+ $4) (with_pc m.(core).(nextPC) m).
+  Proof.
+    intros. reflexivity.
+  Qed.
+  
+  Lemma execState_Return: forall {S A} (s: S) (a: A),
+      execState (Return a) s = s.
+  Proof. intros. reflexivity. Qed.
+
+End AxiomaticRiscv.
+
+Existing Instance State_is_RegisterFile.
